Examples/EdmondsKarp_Maxflow/Graph_Impl.thy
@@ -16,10 +16,17 @@ locale Impl_Succ =
   fixes succ :: "'ga \<Rightarrow> node \<Rightarrow> node list nrest"
   fixes isG :: "'ga \<Rightarrow> 'gi \<Rightarrow> assn"
   fixes succ_impl :: "'gi \<Rightarrow> node \<Rightarrow> node list Heap"
+
+  fixes  set_insert_time map_dom_member_time set_delete_time get_succs_list_time map_update_time set_pick_time :: nat
+    and list_append_time map_lookup_time set_empty_time :: nat
+  assumes [simp]: "map_lookup_time > 0"
+  assumes [simp]: "set_pick_time > 0"
+
   (*assumes [constraint_rules]: "precise isG"*)
   assumes si_rule[sepref_fr_rules]: "(uncurry succ_impl,(uncurry succ)) \<in> [\<lambda>(c,u). u\<in>Graph.V (absG c)]\<^sub>a isG\<^sup>k *\<^sub>a (pure nat_rel)\<^sup>k \<rightarrow> list_assn (pure nat_rel)"
 begin
-  lemma this_loc: "Impl_Succ absG succ isG succ_impl" by unfold_locales
+  lemma this_loc: "Impl_Succ absG succ isG succ_impl map_lookup_time set_pick_time" apply unfold_locales apply simp apply simp 
+    using si_rule .
 
   sepref_register "succ" :: "'ig \<Rightarrow> node \<Rightarrow> node list nrest" (* TODO: Will not work if succ is not a constant! *) 
 end
